Light POC for the `Crypto` library

src/Crypto/HKDF/HMAC.dfy
@@ -2,48 +2,24 @@
 // SPDX-License-Identifier: Apache-2.0
 
 include "../../StandardLibrary/StandardLibrary.dfy"
-include "../Model/Aws.Cryptography.PrimitivesAbstract.dfy"
-
-module HMac {
-  import opened Wrappers
-  import opened UInt = StandardLibrary.UInt
-  import Types = AwsCryptographyPrimitivesTypes
-
-  method Digest(input: Types.HMacInput)
-    returns  ( output: Result<seq<uint8>, Types.Error> )
-  {
-
-  }
-}
-
+include "../Model/AwsCryptographyPrimitivesTypes.dfy"
+include "../Digest.dfy"
 
 module {:extern "HMAC"} HMAC {
   import opened StandardLibrary
   import opened UInt = StandardLibrary.UInt
-
-  datatype {:extern "Digests"} Digests = 
-    | SHA_256
-    | SHA_384
-    | SHA_512
-
-  // Hash length in octets (bytes), e.g. GetHashLength(SHA_256) ==> 256 bits = 32 bytes ==> n = 32
-  function method GetHashLength(digest: Digests): int
-  {
-    match digest
-    case SHA_256 => 32
-    case SHA_384 => 48
-    case SHA_512 => 64
-  }
+  import Types = AwsCryptographyPrimitivesTypes
+  import Digest
 
   class {:extern "HMac"} HMac {
 
     // These functions are used to model the extern state
     // https://github.com/dafny-lang/dafny/wiki/Modeling-External-State-Correctly
     function {:extern} GetKey(): seq<uint8> reads this
-    function {:extern} GetDigest(): Digests reads this
+    function {:extern} GetDigest(): Types.DigestAlgorithm reads this
     function {:extern} GetInputSoFar(): seq<uint8> reads this
 
-    constructor {:extern} (digest: Digests)
+    constructor {:extern} (digest: Types.DigestAlgorithm)
       ensures this.GetDigest() == digest
       ensures this.GetInputSoFar() == []
 
@@ -64,7 +40,7 @@ module {:extern "HMAC"} HMAC {
     method {:extern "GetResult"} GetResult() returns (s: seq<uint8>)
       requires |this.GetKey()| > 0
       modifies this
-      ensures |s| == GetHashLength(this.GetDigest())
+      ensures |s| == Digest.Length(this.GetDigest())
       ensures this.GetInputSoFar() == []
       ensures this.GetDigest() == old(this.GetDigest())
       ensures this.GetKey() == old(this.GetKey())
