src/Crypto/WrappedHKDF.dfy
@@ -1,0 +1,39 @@
+// Copyright Amazon.com Inc. or its affiliates. All Rights Reserved.
+// SPDX-License-Identifier: Apache-2.0
+
+include "HKDF/HKDF.dfy"
+include "HKDF/HMAC.dfy"
+include "Model/AwsCryptographyPrimitivesTypes.dfy"
+
+/*
+ * Implementation of the https://tools.ietf.org/html/rfc5869 HMAC-based key derivation function
+ */
+module Wrapped {
+  import opened Wrappers
+  import opened UInt = StandardLibrary.UInt
+  import Types = AwsCryptographyPrimitivesTypes
+  import HMAC
+  import HKDF
+
+  method Extract(input: Types.HkdfExtractInput) returns (prk: seq<uint8>)
+  {
+    var HkdfExtractInput(digest, salt, ikm) := input;
+  }
+
+  method Expand(input: Types.HkdfExpandInput) returns (okm: seq<uint8>)
+  {
+    var HkdfExpandInput(digest, prk, info, expectedLength) := input;
+
+
+  }
+
+  /*
+   * The RFC 5869 KDF. Outputs L bytes of output key material.
+   */
+  method Hkdf(input: Types.HkdfInput) returns (okm: seq<uint8>)
+  {
+    var HkdfInput(digest, salt, ikm, info, expectedLength) := input;
+
+    okm := HKDF.Hkdf(digest, salt, ikm, info, expectedLength);
+  }
+}
