src/Crypto/WrappedHMAC.dfy
@@ -1,0 +1,28 @@
+// Copyright Amazon.com Inc. or its affiliates. All Rights Reserved.
+// SPDX-License-Identifier: Apache-2.0
+
+include "Model/AwsCryptographyPrimitivesTypes.dfy"
+include "HKDF/HMAC.dfy"
+
+module WrappedHMAC {
+  import opened StandardLibrary
+  import opened Wrappers
+  import opened UInt = StandardLibrary.UInt
+  import Types = AwsCryptographyPrimitivesTypes
+  import HMAC
+
+  method Digest(input: Types.HMacInput)
+    returns  ( output: Result<seq<uint8>, Types.Error> )
+  {
+    var HMacInput(digestAlgorithm, key, message) := input;
+
+    var hmac := new HMAC.HMac(digestAlgorithm);
+    hmac.Init(key);
+    hmac.Update(message);
+    var value := hmac.GetResult();
+
+    // Any runtime Need check go here
+
+    return Success(value);
+  }
+}
